Generated the initial proof structure for proving phinode-elimination.
1) the design structure of phinode-elim is similar to the design of
elim_stld loops. So, we first represent the structure in iter_pass.v,
whose correctness is in iter_pass_correct.v. Both the existent proofs of
elim_stld in mem2reg_correct.v and the incoming proofs in phielim_top.v
are instances of iter_pass_correct.v. 

Actually, the macro_mem2reg_fdef_step (the top-level loop) also follows
the same structure. We should instantiate it later.

2) To deal with the same issue we discussed in r3974, phielim pass also
only checks reachable blocks. Since we only inserted phinodes in
reachable blocks, the restriction wont remove less phi-nodes.
Experiments also confirmed the claim.

3) The initial proof structure of phielim is in phielim_top.v. 

In high-level, the pass is a pipe-line of composition of substitution
followed by DIE.

In middle-level, tasks to do.

task1.1: extend die.v to allow removing phinodes
task1.2: prove the specification of phielim pass to get its declarative
properties, which are more convenient for proofs.

task2.1: prove that x = phi x x x x cannot appear in reachable blocks
task2.2: prove that in x = phi x v x v x where x <> v, v strictly dominates x 
         if x reachable.

task3.1: prove that subst x by v in tasks 2.2 preserves WF. subst_wf.v
          proves this trivially. 
task3.2: prove that subst x by v in tasks 2.2 preserves semantics.
          
We need one more step before finishing constructing proof structure. task3.2 
will be refined. The proof structure of substituting phinodes should be same to 
las/laa, which needs two steps

 a) prove that the input program has the invariant for x and v: 
    when x and v are in scope, they equal.
 b) prove that if the invariant holds, subsitution preserves semantics.

For las/laa/phielim, their b) are the same, a) are different. We will
first define a module for b), then task3.2 will only be focused on a).

4) To test pruned SSA, we should check 129.compress, which leads to
observable performance gap, than in the output, there are more unpruned
phinodes than other testcases.



git-svn-id: https://webdav.seas.upenn.edu/svn/sol/vol@3975 eef5ea85-cc2e-0410-bd84-0fae1f012da8

src3.0/Transforms/mem2reg.v
@@ -6,6 +6,7 @@ Require Import Lattice.
 Require Import Iteration.
 Require Import primitives.
 Require Import dtree.
+Require Import iter_pass.
 
 Record vmap := mkVMap {
   alloca: value;
@@ -328,27 +329,13 @@ match find_init_stld cs pid dones with
     end
 end.
 
-Fixpoint elim_stld_blocks (f:fdef) (bs: blocks) (rd:list l) (pid:id) 
-  (dones:list id) : fdef * bool * list id :=
-match bs with
-| nil => (f, false, dones)
-| block_intro l0 _ cs _::bs' =>
-    if (in_dec id_dec l0 rd) then
-      let '(f', changed, dones') := elim_stld_cmds f cs pid dones in
-      if changed then (f', true, dones') 
-      else elim_stld_blocks f' bs' rd pid dones
-    else elim_stld_blocks f bs' rd pid dones
+Definition elim_stld_block (f:fdef) (b: block) (pid:id) (dones:list id) 
+  : fdef * bool * list id :=
+match b with
+| block_intro _ _ cs _=> elim_stld_cmds f cs pid dones 
 end.
 
-Definition elim_stld_fdef (f:fdef) (rd:list l) (pid:id) (dones:list id)
-  : fdef * bool * list id :=
-let '(fdef_intro fh bs) := f in elim_stld_blocks f bs rd pid dones.
-
-Definition elim_stld_step (rd:list l) (pid:id) (st: fdef * list id)
-  : fdef * list id + fdef * list id :=
-let '(f, dones) := st in
-let '(f1, changed1, dones1) := elim_stld_fdef f rd pid dones in
-if changed1 then inr _ (f1, dones1) else inl _ (f1, dones1).
+Definition ElimStld := mkIterPass (list id) id elim_stld_block nil.
 
 Parameter does_stld_elim : unit -> bool.
 
@@ -380,7 +367,7 @@ match getEntryBlock f with
         let f1 := phinodes_placement rd pid ty al succs preds f in
         let '(f2, _) :=
           if does_stld_elim tt then
-            SafePrimIter.iterate _ (elim_stld_step rd pid) (f1, nil)
+            IterationPass.iter ElimStld pid rd f1
           else (f1, nil)
         in
         let f3 :=
@@ -446,20 +433,13 @@ match ps with
     if changed then (f', true) else eliminate_phis f' ps'
 end.
 
-Fixpoint eliminate_blocks (f:fdef) (bs: blocks): fdef * bool :=
-match bs with
-| nil => (f, false)
-| block_intro _ ps _ _::bs' =>
-    let '(f', changed) := eliminate_phis f ps in
-    if changed then (f', true) else eliminate_blocks f' bs'
+Definition eliminate_block (f:fdef) (b: block) (ut:unit) (dones:list id) 
+  : fdef * bool * list id :=
+match b with
+| block_intro _ ps _ _=> (eliminate_phis f ps, dones)
 end.
 
-Definition eliminate_fdef (f:fdef) : fdef * bool :=
-let '(fdef_intro fh bs) := f in eliminate_blocks f bs.
-
-Definition eliminate_step (f: fdef) : fdef + fdef :=
-let '(f1, changed1) := eliminate_fdef f  in
-if changed1 then inr _ f1 else inl _ f1.
+Definition ElimPhi := mkIterPass (list id) unit eliminate_block nil.
 
 Parameter does_phi_elim : unit -> bool.
 Parameter does_macro_m2r : unit -> bool.
@@ -538,8 +518,8 @@ match getEntryBlock f, reachablity_analysis f with
         else (f, nil)
     in
     let f2 :=
-      if does_phi_elim tt then SafePrimIter.iterate _ eliminate_step f1
-      else f1 in
+      if does_phi_elim tt 
+      then fst (IterationPass.iter ElimPhi tt rd f1) else f1 in
     match fix_temporary_fdef f2 with
     | Some f' => f'
     | None => f
@@ -556,3 +536,4 @@ module_intro los nts
              | product_fdef f => product_fdef (mem2reg_fdef f)
              | _ => p
              end) ps).
+
