src3.0/Transforms/mem2reg_correct.v
@@ -27,6 +27,9 @@ Require Import sas_top.
 Require Import sas_wfS.
 Require Import phiplacement_bsim_wfS.
 Require Import phiplacement_bsim_top.
+Require Import iter_pass.
+Require Import iter_pass_correct.
+Require Import phielim_top.
 
 (* We are proving the macro-based m2r pass *)
 Parameter does_macro_m2r_is_true: mem2reg.does_macro_m2r tt = true.
@@ -36,31 +39,6 @@ Parameter print_reachablity_is_true: forall rd, print_reachablity rd = true.
 Parameter does_phi_elim_is_true: does_phi_elim tt = true.
 
 Parameter does_stld_elim_is_true: does_stld_elim tt = true.
-
-Lemma program_sim_wfS_trans: forall (P1 P2 P3 : system) (main : id)
-  (VarArgs : list (GVsT DGVs)) (HwfS: wf_system P3) 
-  (Hok: defined_program P3 main VarArgs),
-  (wf_system P2 -> 
-   defined_program P2 main VarArgs ->
-   program_sim P1 P2 main VarArgs /\ wf_system P1 /\ 
-   defined_program P1 main VarArgs) ->
-  (wf_system P3 -> 
-   defined_program P3 main VarArgs ->
-   program_sim P2 P3 main VarArgs /\ wf_system P2 /\
-   defined_program P2 main VarArgs) ->
-  program_sim P1 P3 main VarArgs /\ wf_system P1 /\
-  defined_program P1 main VarArgs.
-Proof.
-  intros.
-  destruct H0 as [Hsim2 [Hwf2 Hok2]]; auto.
-  destruct H as [Hsim1 [Hwf1 Hok1]]; auto.
-  split; auto.
-  eapply program_sim_trans; eauto.
-Qed.
-
-Lemma subst_fdef_PI_f__PI_f_subst_pinfo: forall i1 v pinfo,
-  subst_fdef i1 v (PI_f pinfo) = PI_f (subst_pinfo i1 v pinfo).
-Proof. destruct pinfo; auto. Qed.
 
 Lemma las_die_wfPI: forall (los : layouts) (nts : namedts) (fh : fheader)
   (dones : list id) (pinfo: PhiInfo)
@@ -267,6 +245,18 @@ Proof.
       eapply program_sim__preserves__defined_program; eauto using laa_sim.
 Qed.
 
+Lemma elim_stld_cmds_unchanged: forall f' dones' f cs0 pid dones,
+  (f', false, dones') = elim_stld_cmds f cs0 pid dones ->
+  f' = f /\ dones = dones'.
+Proof.
+  intros.
+  unfold elim_stld_cmds in H.
+  destruct (find_init_stld cs0 pid dones) as [[[[]]|[]]|].
+    destruct (find_next_stld c pid) as [[|[]]|]; inv H.
+    destruct (find_next_stld c pid) as [[|[]]|]; inv H.
+    inv H; auto.
+Qed.
+
 Lemma remove_subst_reachablity_successors : forall i2 i1 v1 f,
   reachablity_analysis f =
     reachablity_analysis (remove_fdef i2 (subst_fdef i1 v1 f)) /\
@@ -305,27 +295,6 @@ Proof.
       split; auto.
       split; auto.
 Qed.
-
-Definition keep_pinfo (f:fdef) (pinfo1 pinfo2: PhiInfo) :=
-PI_f pinfo2 = f /\
-PI_rd pinfo1 = PI_rd pinfo2 /\
-PI_id pinfo1 = PI_id pinfo2 /\
-PI_typ pinfo1 = PI_typ pinfo2 /\
-PI_align pinfo1 = PI_align pinfo2.
-
-Hint Unfold keep_pinfo.
-
-Ltac instantiate_pinfo :=
-match goal with
-| HwfS : WF_PhiInfo (update_pinfo ?f ?pi) |- _ => 
-  exists (update_pinfo f pi); repeat (split; auto)
-| HwfS : WF_PhiInfo ?pi, Heq: (PI_f ?pi) = ?f |- 
-  exists _ : _, WF_PhiInfo _ /\ keep_pinfo ?f ?pi _ =>
-  rewrite <- Heq; exists pi; repeat (split; auto)
-| HwfS : WF_PhiInfo ?pi |- 
-  exists _ : _, WF_PhiInfo _ /\ keep_pinfo (PI_f ?pi) ?pi _ =>
-  exists pi; repeat (split; auto)
-end.
 
 Lemma elim_stld_cmds_wfPI: forall los nts fh dones (pinfo:PhiInfo) f0 dones0
   bs1 l0 ps0 cs0 tmn0 bs2 Ps1 Ps2 (Hreach:  In l0 (PI_rd pinfo))
@@ -401,264 +370,22 @@ Proof.
       split; auto using program_sim_refl.
 Qed.
 
-Ltac elim_stld_blocks_tac :=
-repeat match goal with
-| H1: context [?A ++ block_intro ?l0 ?ps0 ?cs0 ?tmn0 :: ?C] |- _ => 
-      rewrite_env ((A++[block_intro l0 ps0 cs0 tmn0])++C) in H1
-| |- context [?A ++ block_intro ?l0 ?ps0 ?cs0 ?tmn0 :: ?C] => 
-      rewrite_env ((A++[block_intro l0 ps0 cs0 tmn0])++C)
-| H1:forall _:_, _ -> _ |- _ => progress (eapply H1; eauto)
-end.
-
-Lemma elim_stld_blocks_reachablity_successors_aux: forall f0 dones0 dones id0
-  flag fh rd bs2 bs1
-  (Hpass:elim_stld_blocks (fdef_intro fh (bs1++bs2)) bs2 rd id0 dones =
-    (f0, flag, dones0)),
-  reachablity_analysis (fdef_intro fh (bs1++bs2)) =
-    reachablity_analysis f0 /\
-  successors (fdef_intro fh (bs1++bs2)) = successors f0.
-Proof.
-  induction bs2; simpl; intros.
-    inv Hpass. auto.
-
-    destruct a as [l0 ps0 cs0 tmn0].
-    destruct (in_dec id_dec l0 rd).
-    Case "reachable".
-      remember
-        (elim_stld_cmds
-          (fdef_intro fh (bs1 ++ block_intro l0 ps0 cs0 tmn0 :: bs2))
-            cs0 id0 dones) as R.
-      destruct R as [[f' []] dones']; inv Hpass; auto.
-        eapply elim_stld_cmds_reachablity_successors; eauto.
-
-        apply elim_stld_cmds_unchanged in HeqR. subst.
-        elim_stld_blocks_tac.
-
-    Case "unreachable". 
-      elim_stld_blocks_tac.
-Qed.
-
-Lemma elim_stld_blocks_wfPI_aux: forall los nts fh dones (pinfo:PhiInfo) f0
-  dones0 Ps1 Ps2 flag bs2 bs1
-  (Hpass:elim_stld_blocks (fdef_intro fh (bs1++bs2)) bs2 (PI_rd pinfo) 
-    (PI_id pinfo) dones = (f0, flag, dones0))
-  (Heq: PI_f pinfo = fdef_intro fh (bs1 ++ bs2))
-  (Hwfpi: WF_PhiInfo pinfo)
-  (HwfS :
-     wf_system
-       [module_intro los nts
-         (Ps1 ++
-          product_fdef
-            (fdef_intro fh (bs1 ++ bs2)) :: Ps2)]),
-  exists pinfo', WF_PhiInfo pinfo' /\ keep_pinfo f0 pinfo pinfo'.
-Proof.
-  induction bs2; simpl; intros.
-    inv Hpass. instantiate_pinfo.
-
-    destruct a as [l0 ps0 cs0 tmn0].
-    destruct (in_dec id_dec l0 (PI_rd pinfo)).
-    Case "reachable".
-      remember
-        (elim_stld_cmds
-          (fdef_intro fh (bs1 ++ block_intro l0 ps0 cs0 tmn0 :: bs2))
-            cs0 (PI_id pinfo) dones) as R.
-      destruct R as [[f' []] dones']; inv Hpass; auto.
-        eapply elim_stld_cmds_wfPI; eauto.
-
-        apply elim_stld_cmds_unchanged in HeqR; subst.
-        elim_stld_blocks_tac.
-    Case "unreachable". 
-      elim_stld_blocks_tac.
-Qed.
-
-Lemma elim_stld_blocks_sim_wfS_aux: forall los nts fh dones (pinfo:PhiInfo) f0
-  dones0 main VarArgs Ps1 Ps2 flag bs2 bs1
-  (Hpass:elim_stld_blocks (fdef_intro fh (bs1++bs2)) bs2 (PI_rd pinfo)
-    (PI_id pinfo) dones = (f0, flag, dones0))
-  (Heq: PI_f pinfo = fdef_intro fh (bs1 ++ bs2))
-  (Hwfpi: WF_PhiInfo pinfo) S1 S2
-  (Heq1: S1 = [module_intro los nts (Ps1 ++  product_fdef f0 :: Ps2)])
-  (heq2: S2 = [module_intro los nts
-      (Ps1 ++ product_fdef (fdef_intro fh (bs1++bs2)) :: Ps2)])
-  (HwfS : wf_system S2) (Hok: defined_program S2 main VarArgs),
-  program_sim S1 S2 main VarArgs /\ wf_system S1 /\
-    defined_program S1 main VarArgs.
-Proof.
-  induction bs2; simpl; subst; intros.
-    inv Hpass; split; auto using program_sim_refl.
-
-    destruct a as [l0 ps0 cs0 tmn0].
-    destruct (in_dec id_dec l0 (PI_rd pinfo)).
-    Case "reachable".
-      remember
-        (elim_stld_cmds
-          (fdef_intro fh (bs1 ++ block_intro l0 ps0 cs0 tmn0 :: bs2))
-            cs0 (PI_id pinfo) dones) as R.
-      destruct R as [[f' []] dones']; inv Hpass; auto.
-        eapply elim_stld_cmds_sim_wfS; eauto.
-
-        apply elim_stld_cmds_unchanged in HeqR. subst.
-        elim_stld_blocks_tac.
-    Case "unreachable". 
-      elim_stld_blocks_tac.
-Qed.
-
-Lemma elim_stld_blocks_reachablity_successors: forall f0 dones0 dones id0
-  flag fh bs rd
-  (Hpass:elim_stld_blocks (fdef_intro fh bs) bs rd id0 dones =
-    (f0, flag, dones0)),
-  reachablity_analysis (fdef_intro fh bs) =
-    reachablity_analysis f0 /\
-  successors (fdef_intro fh bs) = successors f0.
-Proof.
-  intros.
-  rewrite_env (nil ++ bs).
-  eapply elim_stld_blocks_reachablity_successors_aux; eauto.
-Qed.
-
-Lemma elim_stld_blocks_wfPI: forall los nts fh dones (pinfo:PhiInfo) f0 dones0
-  Ps1 Ps2 flag bs
-  (Hpass:elim_stld_blocks (fdef_intro fh bs) bs (PI_rd pinfo) (PI_id pinfo) 
-           dones = (f0, flag, dones0))
-  (Heq: PI_f pinfo = fdef_intro fh bs)
-  (Hwfpi: WF_PhiInfo pinfo)
-  (HwfS :
-     wf_system
-       [module_intro los nts
-         (Ps1 ++ product_fdef (fdef_intro fh bs) :: Ps2)]),
-  exists pinfo', WF_PhiInfo pinfo' /\ keep_pinfo f0 pinfo pinfo'.
-Proof.
-  intros.
-  rewrite_env (nil ++ bs) in HwfS.
-  eapply elim_stld_blocks_wfPI_aux; eauto; simpl; eauto.
-Qed.
-
-Lemma elim_stld_blocks_sim_wfS: forall los nts fh dones (pinfo:PhiInfo) f0 dones0
-  main VarArgs Ps1 Ps2 flag bs
-  (Hpass:elim_stld_blocks (fdef_intro fh bs) bs (PI_rd pinfo) (PI_id pinfo) dones
-           = (f0, flag, dones0))
-  (Heq: PI_f pinfo = fdef_intro fh bs)
-  (Hwfpi: WF_PhiInfo pinfo) S1 S2
-  (Heq1: S1 = [module_intro los nts (Ps1 ++  product_fdef f0 :: Ps2)])
-  (Heq2: S2 = [module_intro los nts (Ps1 ++ product_fdef (fdef_intro fh bs) :: Ps2)])
-  (HwfS : wf_system S2) (Hok: defined_program S2 main VarArgs), 
-  program_sim S1 S2 main VarArgs /\ wf_system S1 /\ defined_program S1 main VarArgs.
-Proof.
-  intros until bs.
-  rewrite_env (nil ++ bs).
-  intros. subst.
-  eapply elim_stld_blocks_sim_wfS_aux; eauto.
-Qed.
-
-Lemma elim_stld_sim_reachablity_successors: forall f1 dones1 f2 dones2 rd pid
-  (Hpass: SafePrimIter.iterate _ (elim_stld_step rd pid) (f1, dones1) =
-    (f2, dones2)),
-  reachablity_analysis f2 = reachablity_analysis f1 /\
-  successors f2 = successors f1.
-Proof.
-  intros. subst.
-  set (P:=fun (re:(fdef * list id)) =>
-          let '(f, _) := re in
-          reachablity_analysis f = reachablity_analysis f1 /\
-          successors f = successors f1).
-  assert (P (f1, dones1)) as HPf1.
-    unfold P. split; auto.
-  apply SafePrimIter.iterate_prop with (P:=P) in Hpass; auto.
-    unfold elim_stld_step.
-    intros a HPa.
-    destruct a as [f dones].
-    unfold elim_stld_fdef.
-    destruct f as [fh bs].
-    remember (elim_stld_blocks (fdef_intro fh bs) bs rd pid dones) as R.
-    destruct R as [[f0 flag0] dones0]; auto.
-    assert (P (f0, dones0)) as HPf0.
-      unfold P.
-      symmetry in HeqR.
-      apply elim_stld_blocks_reachablity_successors in HeqR.
-      destruct HeqR. destruct HPa.
-      split.
-        transitivity (reachablity_analysis (fdef_intro fh bs)); auto.
-        transitivity (successors (fdef_intro fh bs)); auto.
-
-    destruct flag0; auto.
-Qed.
-
-Lemma keep_pinfo_trans: forall f f' p1 p2 p3
-  (H1: keep_pinfo f p1 p2) (H2: keep_pinfo f' p2 p3),
-  keep_pinfo f' p1 p3.
-Proof.
-  intros.
-  destruct H1 as [A [B [C [D E]]]].
-  destruct H2 as [A' [B' [C' [D' E']]]].
-  repeat split; try solve [auto | etransitivity; eauto].
-Qed.
-
-Lemma change_keep_pinfo: forall f pinfo1 pinfo2
-  (H1: PI_id pinfo1 = PI_id pinfo2)
-  (H2: PI_typ pinfo1 = PI_typ pinfo2)
-  (H3: PI_align pinfo1 = PI_align pinfo2)
-  (H4: PI_rd pinfo1 = PI_rd pinfo2),
-  (exists pinfo' : PhiInfo, WF_PhiInfo pinfo' /\ keep_pinfo f pinfo1 pinfo') -> 
-  exists pinfo' : PhiInfo, WF_PhiInfo pinfo' /\ keep_pinfo f pinfo2 pinfo'.
-Proof.
-  intros.
-  destruct H as [A [B C]].
-  exists A. split; auto.
-  unfold keep_pinfo in *.
-  rewrite <- H1. rewrite <- H2. rewrite <- H3. rewrite <- H4. auto.
-Qed.
-
-Lemma update_pinfo_refl: forall f0 pinfo pinfo' 
-  (Hkp: keep_pinfo f0 pinfo pinfo'), (update_pinfo pinfo' f0) = pinfo'.
-Proof.
-  intros.
-  destruct Hkp as [EQ _]; subst. destruct pinfo'. auto.
-Qed.
-
-Ltac solve_keep_pinfo :=
+Ltac elim_stld_block_tac :=
+intros;
 match goal with
-| Hkeep : keep_pinfo _ ?pinfo ?pinfo' |- PI_id ?pinfo' = PI_id ?pinfo =>
-  destruct Hkeep as [? [? [? ?]]]; auto
-| Hkeep : keep_pinfo _ ?pinfo ?pinfo' |- PI_rd ?pinfo' = PI_rd ?pinfo =>
-  destruct Hkeep as [? [? [? ?]]]; auto
-| Hkeep : keep_pinfo ?f ?pinfo ?pinfo' |- PI_f ?pinfo' = ?f =>
-  destruct Hkeep as [? ?]; auto
-| Hkeep : keep_pinfo ?f1 ?pinfo ?pinfo',
-  HeqR : exists _:_,
-            WF_PhiInfo _ /\ keep_pinfo ?f0 ?pinfo' _ |-
-  exists _:_, WF_PhiInfo _ /\ keep_pinfo ?f0 ?pinfo _ =>
-  let A:=fresh "A" in
-  destruct HeqR as [A [? ?]];
-  exists A; split; auto; apply keep_pinfo_trans with (f:=f1)(p2:=pinfo'); auto
-| G: exists _:_, WF_PhiInfo _ /\ keep_pinfo ?f (update_pinfo ?pi _) _ |-
-  exists _:_, WF_PhiInfo _ /\ keep_pinfo ?f ?pi _ =>
-  let A:=fresh "A" in
-  destruct G as [A [? ?]]; exists A; split; auto
-| pinfo := {|
-           PI_f := _;
-           PI_rd := _;
-           PI_id := ?pid;
-           PI_typ := _;
-           PI_num := _;
-           PI_align := _ |} : PhiInfo, 
-  Hkeep : keep_pinfo _ ?pinfo ?pinfo' |- PI_id ?pinfo' = ?pid =>
-  destruct Hkeep as [? [? [? ?]]]; auto
-| pinfo := {|
-           PI_f := _;
-           PI_rd := _;
-           PI_id := ?pid;
-           PI_typ := _;
-           PI_num := _;
-           PI_align := _ |} : PhiInfo, 
-  Hkeep : keep_pinfo _ ?pinfo ?pinfo' |- ?pid = PI_id ?pinfo' =>
-  destruct Hkeep as [? [? [? ?]]]; auto
-| H: ?f _ _ = ?e |- ?f _ _ = ?e => rewrite H; f_equal; solve_keep_pinfo
-| H: ?e = ?f _ _ |- ?f _ _ = ?e => rewrite H; f_equal; solve_keep_pinfo
+| H:context [iter_block ElimStld _ ?b0 _ _] |- _ => destruct b0; simpl in H; 
+  try solve [
+    eapply elim_stld_cmds_unchanged; eauto 2 |
+    eapply elim_stld_cmds_wfPI; eauto 2 |
+    eapply elim_stld_cmds_sim_wfS; eauto 2 |
+    eapply elim_stld_cmds_reachablity_successors; eauto 2
+  ]
+| _ => solve_keep_pinfo
 end.
 
-Lemma elim_stld_sim_wfS_wfPI: forall f1 dones1 f2 dones2 Ps1 Ps2 los nts main
-  VarArgs pid rd (pinfo:PhiInfo)
-  (Hpass: SafePrimIter.iterate _ (elim_stld_step rd pid)
+Lemma elim_stld_sim_wfS_wfPI: forall f1 f2 Ps1 Ps2 los nts main
+  VarArgs pid rd (pinfo:PhiInfo) (dones1 dones2:ElimStld.(effects))
+  (Hpass: SafePrimIter.iterate _ (IterationPass.iter_step ElimStld pid rd)
     (f1, dones1) = (f2, dones2))
   (Heq1: PI_f pinfo = f1) (Heq2: PI_id pinfo = pid) (Heq2: PI_rd pinfo = rd)
   (Hwfpi: WF_PhiInfo pinfo) S1 S2
@@ -669,48 +396,13 @@ Lemma elim_stld_sim_wfS_wfPI: forall f1 dones1 f2 dones2 Ps1 Ps2 los nts main
     defined_program S1 main VarArgs) /\
   exists pinfo', WF_PhiInfo pinfo' /\ keep_pinfo f2 pinfo pinfo'.
 Proof.
-  intros. subst.
-  set (P:=fun (re:(fdef * list id)) =>
-          let '(f, _) := re in
-          (program_sim [module_intro los nts (Ps1 ++ product_fdef f :: Ps2)]
-            [module_intro los nts (Ps1 ++ product_fdef (PI_f pinfo) :: Ps2)]
-            main VarArgs /\
-           wf_system
-            [module_intro los nts (Ps1 ++ product_fdef f :: Ps2)] /\
-           defined_program 
-            [module_intro los nts (Ps1 ++ product_fdef f :: Ps2)]
-            main VarArgs) /\
-          exists pinfo', WF_PhiInfo pinfo' /\ keep_pinfo f pinfo pinfo'
-       ).
-  assert (P (PI_f pinfo, dones1)) as HPf1.
-    unfold P.
-    split; auto using program_sim_refl. instantiate_pinfo.
-  apply SafePrimIter.iterate_prop with (P:=P) in Hpass; auto.
-    unfold elim_stld_step.
-    intros a HPa.
-    destruct a as [f dones].
-    unfold elim_stld_fdef.
-    destruct f as [fh bs].
-    remember (elim_stld_blocks (fdef_intro fh bs) bs 
-               (PI_rd pinfo) (PI_id pinfo) dones) as R.
-    destruct R as [[f0 flag0] dones0]; auto.
-    assert (P (f0, dones0)) as HPf0.
-      unfold P.
-      symmetry in HeqR.
-      destruct HPa as 
-        [[Hsima [HwfSa Hoka]] [pinfo' [HwfPIa Hkeep]]].
-      replace (PI_id pinfo) with (PI_id pinfo') in HeqR; try solve_keep_pinfo.
-      replace (PI_rd pinfo) with (PI_rd pinfo') in HeqR; try solve_keep_pinfo.
-      split.
-        apply program_sim_wfS_trans with (P2:=
-                [module_intro los nts
-                 (Ps1 ++ product_fdef (fdef_intro fh bs) :: Ps2)]); auto.
-          intros.
-          eapply elim_stld_blocks_sim_wfS in HeqR; eauto; try solve_keep_pinfo.
-        eapply elim_stld_blocks_wfPI in HeqR; eauto; try solve_keep_pinfo.
-
-    destruct flag0; auto.
+  intros. 
+  eapply IterationPassCorrect.iter_wfS_wfPI; eauto.
+    elim_stld_block_tac. elim_stld_block_tac. 
+    elim_stld_block_tac. elim_stld_block_tac. 
 Qed.
+
+Hint Unfold keep_pinfo.
 
 Lemma macro_mem2reg_fdef_sim_wfS: forall rd f1 dones1 f2 dones2 Ps1 Ps2 los
   nts main VarArgs (Hreach: ret rd = reachablity_analysis f1)
@@ -760,11 +452,11 @@ Proof.
       eapply find_promotable_alloca__WF_PhiInfo; eauto.
 
     rewrite does_stld_elim_is_true.
-    remember (SafePrimIter.iterate (fdef * list id)
-               (elim_stld_step rd pid)
+    remember (IterationPass.iter ElimStld pid rd
                (phinodes_placement rd pid ty al (successors f1)
-               (make_predecessors (successors f1)) f, nil)) as R.
+                  (make_predecessors (successors f1)) f)) as R.
     destruct R as [f0 dones0].
+    unfold IterationPass.iter in HeqR1.
 
     assert (P (f0, dones0)) as HPf0.
       symmetry in HeqR1.
@@ -794,7 +486,9 @@ Proof.
               eauto using phinodes_placement_sim.          
 
       Case "2".
-        apply elim_stld_sim_reachablity_successors in HeqR1.
+        apply IterationPassCorrect.iter_reachablity_successors in HeqR1; 
+          try solve [auto | elim_stld_block_tac]. 
+
         destruct HeqR1.
         split.
           transitivity (reachablity_analysis
@@ -818,7 +512,7 @@ Proof.
                    (make_predecessors (successors f)) f))); auto.
      destruct HPa as [HPa1 [HPa2 HPa3]].
      eapply elim_stld_sim_wfS_wfPI; eauto.
-       rewrite EQ1. auto.
+       simpl. rewrite EQ1. auto.
        eapply phinodes_placement_wfPI; eauto.
        rewrite EQ1. simpl. eapply phinodes_placement_wfS; eauto.
        eapply program_sim__preserves__defined_program; eauto.
@@ -902,15 +596,6 @@ Proof.
         apply remove_successors; auto.
 Qed.
 
-Lemma eliminate_phis_sim_wfS: forall f Ps1 Ps2 los nts main VarArgs
-  S1 S2 (HwfS : wf_system S2) (Hok: defined_program S2 main VarArgs)
-  (Heq1: S1 = [module_intro los nts 
-      (Ps1 ++ product_fdef (SafePrimIter.iterate fdef eliminate_step f) :: Ps2)])
-  (Heq2: S2 = [module_intro los nts (Ps1 ++ product_fdef f :: Ps2)]),
-  program_sim S1 S2 main VarArgs /\ wf_system S1 /\
-    defined_program S1 main VarArgs.
-Admitted. (* From previous work PhiElim [2000] *)
-
 Axiom fix_temporary_fdef_sim_wfS: forall f1 f2 Ps1 Ps2 los nts main VarArgs
   (Hpass: ret f2 = fix_temporary_fdef f1) S1 S2
   (Heq1: S1 = [module_intro los nts (Ps1 ++ product_fdef f2 :: Ps2)])
@@ -924,9 +609,9 @@ Axiom remove_dbg_declares_sim_wfS: forall cs Ps1 Ps2 los nts main
   (Heq2: S2 = [module_intro los nts (Ps1 ++ product_fdef f :: Ps2)])
   (Heq1: S1 = [module_intro los nts 
                  (Ps1 ++ product_fdef (remove_dbg_declares f cs) :: Ps2)]),
-  (program_sim S2 S2 main VarArgs /\
-   wf_system S2 /\
-   defined_program S2 main VarArgs) ->
+  program_sim S2 S2 main VarArgs ->
+  wf_system S2 ->
+  defined_program S2 main VarArgs ->
   program_sim S1 S2 main VarArgs /\ wf_system S1 /\
     defined_program S1 main VarArgs.
 
@@ -959,17 +644,27 @@ Proof.
                    ((remove_dbg_declares f cs), nil)) as R.
   destruct R as [f1 dones]; auto using program_sim_refl.
   rewrite does_phi_elim_is_true.
-  remember (fix_temporary_fdef (SafePrimIter.iterate fdef eliminate_step f1))
+  remember (fix_temporary_fdef (fst (IterationPass.iter ElimPhi tt rd f1)))
     as R.
   destruct R as [f2|]; auto using program_sim_refl.
   apply program_sim_wfS_trans with (P2:=
     [module_intro los nts (Ps1 ++ product_fdef f1 :: Ps2)]); auto; intros.
     apply program_sim_wfS_trans with (P2:=
       [module_intro los nts
-        (Ps1 ++ product_fdef (SafePrimIter.iterate fdef eliminate_step f1)
+        (Ps1 ++ product_fdef (fst (IterationPass.iter ElimPhi tt rd f1))
           :: Ps2)]); auto; intros.
       eapply fix_temporary_fdef_sim_wfS; eauto.
-      eapply eliminate_phis_sim_wfS; eauto.
+      eapply elimphi_sim_wfS with (f:=f1); eauto.
+        assert (reachablity_analysis f = 
+          reachablity_analysis (remove_dbg_declares f cs)) as Hreacheq.
+          eapply remove_dbg_declares_sim_reachablity_successors; eauto.
+        eapply remove_dbg_declares_sim_wfS in HwfS; eauto using program_sim_refl.
+        destruct HwfS as [Hpsim [HwfS Hdefined]].
+        eapply macro_mem2reg_fdef_sim_wfS with (f1:=remove_dbg_declares f cs) 
+          in HwfS; eauto.
+          destruct HwfS as [_ [Hreach _]]. congruence.
+          congruence.
+
   apply program_sim_wfS_trans with (P2:=
     [module_intro los nts 
        (Ps1 ++ product_fdef (remove_dbg_declares f cs) :: Ps2)]); auto; intros.
