src3.0/Transforms/iter_pass.v
@@ -1,0 +1,46 @@
+Require Import vellvm.
+Require Import Iteration.
+
+Structure IterPass := mkIterPass {
+  effects: Type;
+  context: Type;
+  iter_block : fdef -> block -> context -> effects -> fdef * bool * effects;
+  init_effects: effects
+}.
+
+Module IterationPass.
+
+Section IterationPass. 
+
+Variable (pass:IterPass).
+
+Fixpoint iter_blocks (f:fdef) (bs: blocks) (ctx:pass.(context)) (rd:list l) 
+  (efs:pass.(effects)) : fdef * bool * pass.(effects) :=
+match bs with
+| nil => (f, false, efs)
+| b::bs' =>
+    if (in_dec id_dec (getBlockLabel b) rd) then
+      let '(f', changed, efs') := pass.(iter_block) f b ctx efs in
+      if changed then (f', true, efs') 
+      else iter_blocks f' bs' ctx rd efs'
+    else iter_blocks f bs' ctx rd efs
+end.
+
+Definition iter_fdef (f:fdef) (ctx:pass.(context)) (rd:list l)  
+  (efs:pass.(effects)) : fdef * bool * pass.(effects) :=
+let '(fdef_intro fh bs) := f in iter_blocks f bs ctx rd efs.
+
+Definition iter_step (ctx:pass.(context)) (rd:list l) (st: fdef * pass.(effects))
+  : fdef * pass.(effects) + fdef * pass.(effects) :=
+let '(f, efs) := st in
+let '(f1, changed1, efs1) := iter_fdef f ctx rd efs in
+if changed1 then inr _ (f1, efs1) else inl _ (f1, efs1).
+
+Definition iter (ctx:pass.(context)) (rd:list l) (f:fdef) 
+  : fdef * pass.(effects) := 
+SafePrimIter.iterate _ (iter_step ctx rd) (f, pass.(init_effects)).
+
+End IterationPass.
+End IterationPass.
+
+
