src3.0/Transforms/iter_pass_correct.v
@@ -1,0 +1,528 @@
+Require Import vellvm.
+Require Import Iteration.
+Require Import iter_pass.
+Require Import program_sim.
+Require Import palloca_props.
+
+(**********************************************************)
+
+Definition keep_pinfo (f:fdef) (pinfo1 pinfo2: PhiInfo) :=
+PI_f pinfo2 = f /\
+PI_rd pinfo1 = PI_rd pinfo2 /\
+PI_id pinfo1 = PI_id pinfo2 /\
+PI_typ pinfo1 = PI_typ pinfo2 /\
+PI_align pinfo1 = PI_align pinfo2.
+
+Hint Unfold keep_pinfo.
+
+Ltac instantiate_pinfo :=
+match goal with
+| HwfS : WF_PhiInfo (update_pinfo ?f ?pi) |- _ => 
+  exists (update_pinfo f pi); repeat (split; auto)
+| HwfS : WF_PhiInfo ?pi, Heq: (PI_f ?pi) = ?f |- 
+  exists _ : _, WF_PhiInfo _ /\ keep_pinfo ?f ?pi _ =>
+  rewrite <- Heq; exists pi; repeat (split; auto)
+| HwfS : WF_PhiInfo ?pi |- 
+  exists _ : _, WF_PhiInfo _ /\ keep_pinfo (PI_f ?pi) ?pi _ =>
+  exists pi; repeat (split; auto)
+end.
+
+Lemma keep_pinfo_trans: forall f f' p1 p2 p3
+  (H1: keep_pinfo f p1 p2) (H2: keep_pinfo f' p2 p3),
+  keep_pinfo f' p1 p3.
+Proof.
+  intros.
+  destruct H1 as [A [B [C [D E]]]].
+  destruct H2 as [A' [B' [C' [D' E']]]].
+  repeat split; try solve [auto | etransitivity; eauto].
+Qed.
+
+Lemma change_keep_pinfo: forall f pinfo1 pinfo2
+  (H1: PI_id pinfo1 = PI_id pinfo2)
+  (H2: PI_typ pinfo1 = PI_typ pinfo2)
+  (H3: PI_align pinfo1 = PI_align pinfo2)
+  (H4: PI_rd pinfo1 = PI_rd pinfo2),
+  (exists pinfo' : PhiInfo, WF_PhiInfo pinfo' /\ keep_pinfo f pinfo1 pinfo') -> 
+  exists pinfo' : PhiInfo, WF_PhiInfo pinfo' /\ keep_pinfo f pinfo2 pinfo'.
+Proof.
+  intros.
+  destruct H as [A [B C]].
+  exists A. split; auto.
+  unfold keep_pinfo in *.
+  rewrite <- H1. rewrite <- H2. rewrite <- H3. rewrite <- H4. auto.
+Qed.
+
+Lemma update_pinfo_refl: forall f0 pinfo pinfo' 
+  (Hkp: keep_pinfo f0 pinfo pinfo'), (update_pinfo pinfo' f0) = pinfo'.
+Proof.
+  intros.
+  destruct Hkp as [EQ _]; subst. destruct pinfo'. auto.
+Qed.
+
+Ltac solve_keep_pinfo :=
+match goal with
+| Hkeep : keep_pinfo _ ?pinfo ?pinfo' |- PI_id ?pinfo = PI_id ?pinfo' =>
+  destruct Hkeep as [? [? [? ?]]]; auto
+| Hkeep : keep_pinfo _ ?pinfo ?pinfo' |- PI_id ?pinfo' = PI_id ?pinfo =>
+  destruct Hkeep as [? [? [? ?]]]; auto
+| Hkeep : keep_pinfo _ ?pinfo ?pinfo' |- PI_rd ?pinfo' = PI_rd ?pinfo =>
+  destruct Hkeep as [? [? [? ?]]]; auto
+| Hkeep : keep_pinfo ?f ?pinfo ?pinfo' |- PI_f ?pinfo' = ?f =>
+  destruct Hkeep as [? ?]; auto
+| Hkeep : keep_pinfo ?f1 ?pinfo ?pinfo',
+  HeqR : exists _:_,
+            WF_PhiInfo _ /\ keep_pinfo ?f0 ?pinfo' _ |-
+  exists _:_, WF_PhiInfo _ /\ keep_pinfo ?f0 ?pinfo _ =>
+  let A:=fresh "A" in
+  destruct HeqR as [A [? ?]];
+  exists A; split; auto; apply keep_pinfo_trans with (f:=f1)(p2:=pinfo'); auto
+| G: exists _:_, WF_PhiInfo _ /\ keep_pinfo ?f (update_pinfo ?pi _) _ |-
+  exists _:_, WF_PhiInfo _ /\ keep_pinfo ?f ?pi _ =>
+  let A:=fresh "A" in
+  destruct G as [A [? ?]]; exists A; split; auto
+| pinfo := {|
+           PI_f := _;
+           PI_rd := _;
+           PI_id := ?pid;
+           PI_typ := _;
+           PI_num := _;
+           PI_align := _ |} : PhiInfo, 
+  Hkeep : keep_pinfo _ ?pinfo ?pinfo' |- PI_id ?pinfo' = ?pid =>
+  destruct Hkeep as [? [? [? ?]]]; auto
+| pinfo := {|
+           PI_f := _;
+           PI_rd := _;
+           PI_id := ?pid;
+           PI_typ := _;
+           PI_num := _;
+           PI_align := _ |} : PhiInfo, 
+  Hkeep : keep_pinfo _ ?pinfo ?pinfo' |- ?pid = PI_id ?pinfo' =>
+  destruct Hkeep as [? [? [? ?]]]; auto
+| H: ?f _ _ = ?e |- ?f _ _ = ?e => rewrite H; f_equal; solve_keep_pinfo
+| H: ?e = ?f _ _ |- ?f _ _ = ?e => rewrite H; f_equal; solve_keep_pinfo
+end.
+
+(**********************************************************)
+
+Module IterationPassCorrect.
+
+Ltac iter_blocks_tac :=
+repeat match goal with
+| H1: context [?A ++ ?b0 :: ?C] |- _ => 
+  match type of b0 with
+  | block => rewrite_env ((A++[b0])++C) in H1
+  end
+| |- context [?A ++ ?b0 :: ?C] => 
+  match type of b0 with
+  | block => rewrite_env ((A++[b0])++C)
+  end
+| H1:forall _:_, _ -> _ |- _ => progress (eapply H1; eauto)
+end.
+
+Section IterationPassCFG.
+
+Variable (pass:IterPass).
+
+Hypothesis iter_block_unchanged: forall f' efs' f b0 ctx efs,
+  (f', false, efs') = pass.(iter_block) f b0 ctx efs ->
+  f' = f /\ efs = efs'.
+
+Hypothesis iter_block_reachablity_successors: forall f b ctx f0
+  efs0 efs (Hpass : (f0, true, efs0) = pass.(iter_block) f b ctx efs),
+  reachablity_analysis f = reachablity_analysis f0 /\
+  successors f = successors f0.
+
+Lemma iter_blocks_reachablity_successors_aux: forall f0 efs0 efs
+  flag fh bs2 bs1 ctx rd
+  (Hpass:IterationPass.iter_blocks pass (fdef_intro fh (bs1++bs2)) bs2 ctx rd efs
+    = (f0, flag, efs0)),
+  reachablity_analysis (fdef_intro fh (bs1++bs2)) =
+    reachablity_analysis f0 /\
+  successors (fdef_intro fh (bs1++bs2)) = successors f0.
+Proof.
+  induction bs2 as [|b0 bs2]; simpl; intros.
+    inv Hpass. auto.
+
+    destruct (in_dec id_dec (getBlockLabel b0) rd).
+    Case "reachable".
+      remember
+        (pass.(iter_block) (fdef_intro fh (bs1 ++ b0 :: bs2)) b0 ctx efs) as R.
+      destruct R as [[f' []] efs']; inv Hpass; auto.
+        eapply iter_block_reachablity_successors; eauto.
+
+        apply iter_block_unchanged in HeqR. destruct HeqR; subst.
+        iter_blocks_tac.
+
+    Case "unreachable". 
+      iter_blocks_tac.
+Qed.
+
+Lemma iter_blocks_reachablity_successors: forall f0 efs0 efs 
+  flag fh bs ctx rd
+  (Hpass:IterationPass.iter_blocks pass (fdef_intro fh bs) bs ctx rd efs =
+    (f0, flag, efs0)),
+  reachablity_analysis (fdef_intro fh bs) =
+    reachablity_analysis f0 /\
+  successors (fdef_intro fh bs) = successors f0.
+Proof.
+  intros.
+  rewrite_env (nil ++ bs).
+  eapply iter_blocks_reachablity_successors_aux; eauto.
+Qed.
+
+Lemma iter_reachablity_successors: forall f1 efs1 f2 efs2 ctx rd
+  (Hpass: SafePrimIter.iterate _ (IterationPass.iter_step pass ctx rd) 
+    (f1, efs1) = (f2, efs2)),
+  reachablity_analysis f2 = reachablity_analysis f1 /\
+  successors f2 = successors f1.
+Proof.
+  intros. subst.
+  set (P:=fun (re:(fdef * pass.(effects))) =>
+          let '(f, _) := re in
+          reachablity_analysis f = reachablity_analysis f1 /\
+          successors f = successors f1).
+  assert (P (f1, efs1)) as HPf1.
+    unfold P. split; auto.
+  apply SafePrimIter.iterate_prop with (P:=P) in Hpass; auto.
+    unfold IterationPass.iter_step.
+    intros a HPa.
+    destruct a as [f dones].
+    unfold IterationPass.iter_fdef.
+    destruct f as [fh bs].
+    remember (IterationPass.iter_blocks pass (fdef_intro fh bs) bs ctx rd dones) 
+      as R.
+    destruct R as [[f0 flag0] dones0]; auto.
+    assert (P (f0, dones0)) as HPf0.
+      unfold P.
+      symmetry in HeqR.
+      apply iter_blocks_reachablity_successors in HeqR.
+      destruct HeqR. destruct HPa.
+      split.
+        transitivity (reachablity_analysis (fdef_intro fh bs)); auto.
+        transitivity (successors (fdef_intro fh bs)); auto.
+
+    destruct flag0; auto.
+Qed.
+
+End IterationPassCFG.
+
+Section IterationPassSimWFP. 
+
+Variable (pass:IterPass).
+
+Hypothesis iter_block_unchanged: forall f' efs' f b0 ctx efs,
+  (f', false, efs') = pass.(iter_block) f b0 ctx efs ->
+  f' = f /\ efs = efs'.
+
+Hypothesis PI_ctx: PhiInfo -> pass.(context).
+
+Variable (los:layouts) (nts:namedts) (Ps1 Ps2: products).
+
+Hypothesis iter_block_wfPI: forall fh efs f0 efs0
+  (pinfo:PhiInfo) (Hwfpi: WF_PhiInfo pinfo)
+  bs1 b0 bs2 (Hreach: In (getBlockLabel b0) (PI_rd pinfo))
+  (Hpass : (f0, true, efs0) =
+           pass.(iter_block) (fdef_intro fh (bs1 ++ b0 :: bs2)) b0 
+             (PI_ctx pinfo) efs)
+  (Heq: PI_f pinfo = fdef_intro fh (bs1 ++ b0 :: bs2))
+  (HwfS :
+     wf_system
+       [module_intro los nts
+         (Ps1 ++ product_fdef (fdef_intro fh (bs1 ++ b0 :: bs2)) :: Ps2)]),
+  exists pinfo', WF_PhiInfo pinfo' /\ keep_pinfo f0 pinfo pinfo'.
+
+Lemma iter_blocks_wfPI_aux: forall fh efs f0 efs0 flag bs2 bs1
+  (pinfo:PhiInfo) (Hwfpi: WF_PhiInfo pinfo)
+  (Hpass:IterationPass.iter_blocks pass (fdef_intro fh (bs1++bs2)) bs2 
+    (PI_ctx pinfo) (PI_rd pinfo) efs = (f0, flag, efs0))
+  (Heq: PI_f pinfo = fdef_intro fh (bs1 ++ bs2))
+  (HwfS :
+     wf_system
+       [module_intro los nts
+         (Ps1 ++
+          product_fdef
+            (fdef_intro fh (bs1 ++ bs2)) :: Ps2)]),
+  exists pinfo', WF_PhiInfo pinfo' /\ keep_pinfo f0 pinfo pinfo'.
+Proof.
+  induction bs2 as [|b0 bs2]; simpl; intros.
+    inv Hpass. instantiate_pinfo.
+
+    destruct (in_dec id_dec (getBlockLabel b0) (PI_rd pinfo)).
+    Case "reachable".
+      remember
+        (pass.(iter_block)
+          (fdef_intro fh (bs1 ++ b0 :: bs2)) b0 (PI_ctx pinfo) efs) as R.
+      destruct R as [[f' []] efs']; inv Hpass; eauto.
+        apply iter_block_unchanged in HeqR. destruct HeqR; subst.
+        iter_blocks_tac.
+    Case "unreachable". 
+      iter_blocks_tac.
+Qed.
+
+Lemma iter_blocks_wfPI: forall fh efs f0 efs0 flag bs
+  (pinfo:PhiInfo) (Hwfpi: WF_PhiInfo pinfo)
+  (Hpass:IterationPass.iter_blocks pass (fdef_intro fh bs) bs 
+    (PI_ctx pinfo) (PI_rd pinfo) efs = (f0, flag, efs0))
+  (Heq: PI_f pinfo = fdef_intro fh bs)
+  (HwfS :
+     wf_system
+       [module_intro los nts
+         (Ps1 ++ product_fdef (fdef_intro fh bs) :: Ps2)]),
+  exists pinfo', WF_PhiInfo pinfo' /\ keep_pinfo f0 pinfo pinfo'.
+Proof.
+  intros.
+  rewrite_env (nil ++ bs) in HwfS.
+  eapply iter_blocks_wfPI_aux; eauto; simpl; eauto.
+Qed.
+
+Hypothesis iter_block_wfS: forall fh efs f0 efs0
+  (pinfo:PhiInfo) (Hwfpi: WF_PhiInfo pinfo)
+  main VarArgs bs1 b0 bs2 (Hreach:In (getBlockLabel b0) (PI_rd pinfo))
+  (Hpass : (f0, true, efs0) =
+           pass.(iter_block) (fdef_intro fh (bs1 ++ b0 :: bs2)) b0 
+             (PI_ctx pinfo) efs)
+  (Heq: PI_f pinfo = fdef_intro fh (bs1 ++ b0 :: bs2)) S1 S2
+  (Heq1: S1 = [module_intro los nts (Ps1 ++ product_fdef f0 :: Ps2)])
+  (Heq1: S2 = 
+    [module_intro los nts
+      (Ps1 ++ product_fdef (fdef_intro fh (bs1 ++ b0 :: bs2)) :: Ps2)])
+  (HwfS : wf_system S2) (Hok: defined_program S2 main VarArgs),
+  program_sim S1 S2 main VarArgs /\ wf_system S1 /\
+    defined_program S1 main VarArgs.
+
+Lemma iter_blocks_sim_wfS_aux: forall fh efs f0 efs0 main VarArgs flag bs2 bs1
+  (pinfo:PhiInfo) (Hwfpi: WF_PhiInfo pinfo)
+  (Hpass:IterationPass.iter_blocks pass (fdef_intro fh (bs1++bs2)) bs2 
+    (PI_ctx pinfo) (PI_rd pinfo) efs = (f0, flag, efs0))
+  (Heq: PI_f pinfo = fdef_intro fh (bs1 ++ bs2))
+  S1 S2
+  (Heq1: S1 = [module_intro los nts (Ps1 ++  product_fdef f0 :: Ps2)])
+  (heq2: S2 = [module_intro los nts
+      (Ps1 ++ product_fdef (fdef_intro fh (bs1++bs2)) :: Ps2)])
+  (HwfS : wf_system S2) (Hok: defined_program S2 main VarArgs),
+  program_sim S1 S2 main VarArgs /\ wf_system S1 /\
+    defined_program S1 main VarArgs.
+Proof.
+  induction bs2 as [|b0 bs2]; simpl; intros.
+    inv Hpass; split; auto using program_sim_refl.
+
+    destruct (in_dec id_dec (getBlockLabel b0) (PI_rd pinfo)).
+    Case "reachable".
+      remember
+        (pass.(iter_block)
+          (fdef_intro fh (bs1 ++ b0 :: bs2)) b0 (PI_ctx pinfo) efs) as R.
+      destruct R as [[f' []] efs']; inv Hpass; eauto.
+        apply iter_block_unchanged in HeqR. destruct HeqR; subst.
+        iter_blocks_tac.
+    Case "unreachable". 
+      iter_blocks_tac.
+Qed.
+
+Lemma iter_blocks_sim_wfS: forall fh efs f0 efs0 main VarArgs flag bs
+  (pinfo:PhiInfo) (Hwfpi: WF_PhiInfo pinfo)
+  (Hpass:IterationPass.iter_blocks pass (fdef_intro fh bs) bs (PI_ctx pinfo) 
+    (PI_rd pinfo) efs = (f0, flag, efs0))
+  (Heq: PI_f pinfo = fdef_intro fh bs)
+  S1 S2
+  (Heq1: S1 = [module_intro los nts (Ps1 ++  product_fdef f0 :: Ps2)])
+  (Heq2: S2 = [module_intro los nts (Ps1 ++ product_fdef (fdef_intro fh bs) :: Ps2)])
+  (HwfS : wf_system S2) (Hok: defined_program S2 main VarArgs), 
+  program_sim S1 S2 main VarArgs /\ wf_system S1 /\ defined_program S1 main VarArgs.
+Proof.
+  intros until bs.
+  rewrite_env (nil ++ bs).
+  intros. subst.
+  eapply iter_blocks_sim_wfS_aux; eauto.
+Qed.
+
+Hypothesis keep_pinfo__PI_ctx: forall f pinfo pinfo',
+  keep_pinfo f pinfo pinfo' -> PI_ctx pinfo = PI_ctx pinfo'.
+
+Lemma iter_wfS_wfPI: forall f1 efs1 f2 efs2 main rd
+  VarArgs ctx (pinfo:PhiInfo) (Hwfpi: WF_PhiInfo pinfo)
+  (Hpass: SafePrimIter.iterate _ (IterationPass.iter_step pass ctx rd) (f1, efs1) 
+    = (f2, efs2))
+  (Heq1: PI_f pinfo = f1) (Heq2: PI_ctx pinfo = ctx) (Heq2: PI_rd pinfo = rd)
+  S1 S2
+  (Heq1: S1 = [module_intro los nts (Ps1 ++ product_fdef f2 :: Ps2)])
+  (Heq2: S2 = [module_intro los nts (Ps1 ++ product_fdef f1 :: Ps2)])
+  (HwfS : wf_system S2) (Hok: defined_program S2 main VarArgs),
+  (program_sim S1 S2 main VarArgs /\ wf_system S1 /\
+    defined_program S1 main VarArgs) /\
+  exists pinfo', WF_PhiInfo pinfo' /\ keep_pinfo f2 pinfo pinfo'.
+Proof.
+  intros. subst.
+  set (P:=fun (re:(fdef * pass.(effects))) =>
+          let '(f, _) := re in
+          (program_sim [module_intro los nts (Ps1 ++ product_fdef f :: Ps2)]
+            [module_intro los nts (Ps1 ++ product_fdef (PI_f pinfo) :: Ps2)]
+            main VarArgs /\
+           wf_system
+            [module_intro los nts (Ps1 ++ product_fdef f :: Ps2)] /\
+           defined_program 
+            [module_intro los nts (Ps1 ++ product_fdef f :: Ps2)]
+            main VarArgs) /\
+          exists pinfo', WF_PhiInfo pinfo' /\ keep_pinfo f pinfo pinfo'
+       ).
+  assert (P (PI_f pinfo, efs1)) as HPf1.
+    unfold P.
+    split; auto using program_sim_refl. instantiate_pinfo.
+  apply SafePrimIter.iterate_prop with (P:=P) in Hpass; auto.
+    unfold IterationPass.iter_step.
+    intros a HPa.
+    destruct a as [f efs].
+    unfold IterationPass.iter_fdef.
+    destruct f as [fh bs].
+    remember (IterationPass.iter_blocks pass (fdef_intro fh bs) bs 
+                (PI_ctx pinfo) (PI_rd pinfo) efs) as R.
+    destruct R as [[f0 flag0] efs0]; auto.
+    assert (P (f0, efs0)) as HPf0.
+      unfold P.
+      symmetry in HeqR.
+      destruct HPa as 
+        [[Hsima [HwfSa Hoka]] [pinfo' [HwfPIa Hkeep]]].
+      replace (PI_rd pinfo) with (PI_rd pinfo') in HeqR; try solve_keep_pinfo.
+      erewrite keep_pinfo__PI_ctx in HeqR; eauto. 
+      split.
+        apply program_sim_wfS_trans with (P2:=
+                [module_intro los nts
+                 (Ps1 ++ product_fdef (fdef_intro fh bs) :: Ps2)]); auto.
+          intros.
+          eapply iter_blocks_sim_wfS in HeqR; eauto; try solve_keep_pinfo.
+        eapply iter_blocks_wfPI in HeqR; eauto; try solve_keep_pinfo.
+
+    destruct flag0; auto.
+Qed.
+
+End IterationPassSimWFP.
+
+Section IterationPassSimWF. 
+
+Variable (pass:IterPass).
+
+Hypothesis iter_block_unchanged: forall f' efs' f b0 ctx efs,
+  (f', false, efs') = pass.(iter_block) f b0 ctx efs ->
+  f' = f /\ efs = efs'.
+
+Variable (los:layouts) (nts:namedts) (Ps1 Ps2: products) (rd:list l) 
+         (ctx:pass.(context)).
+
+Hypothesis iter_block_wfS: forall fh efs f0 efs0
+  main VarArgs bs1 b0 bs2 (Hreach:In (getBlockLabel b0) rd)
+  (Hpass : (f0, true, efs0) =
+           pass.(iter_block) (fdef_intro fh (bs1 ++ b0 :: bs2)) b0 
+             ctx efs) S1 S2
+  (Hrd: reachablity_analysis (fdef_intro fh (bs1 ++ b0 :: bs2)) = Some rd)
+  (Heq1: S1 = [module_intro los nts (Ps1 ++ product_fdef f0 :: Ps2)])
+  (Heq1: S2 = 
+    [module_intro los nts
+      (Ps1 ++ product_fdef (fdef_intro fh (bs1 ++ b0 :: bs2)) :: Ps2)])
+  (HwfS : wf_system S2) (Hok: defined_program S2 main VarArgs),
+  program_sim S1 S2 main VarArgs /\ wf_system S1 /\
+    defined_program S1 main VarArgs.
+
+Lemma iter_blocks_sim_wfS_aux': forall fh efs f0 efs0 main VarArgs flag bs2 bs1
+  (Hpass:IterationPass.iter_blocks pass (fdef_intro fh (bs1++bs2)) bs2 
+     ctx rd efs = (f0, flag, efs0))
+  (Hrd: reachablity_analysis (fdef_intro fh (bs1 ++ bs2)) = Some rd)
+  S1 S2
+  (Heq1: S1 = [module_intro los nts (Ps1 ++  product_fdef f0 :: Ps2)])
+  (heq2: S2 = [module_intro los nts
+      (Ps1 ++ product_fdef (fdef_intro fh (bs1++bs2)) :: Ps2)])
+  (HwfS : wf_system S2) (Hok: defined_program S2 main VarArgs),
+  program_sim S1 S2 main VarArgs /\ wf_system S1 /\
+    defined_program S1 main VarArgs.
+Proof.
+  induction bs2 as [|b0 bs2]; simpl; intros.
+    inv Hpass; split; auto using program_sim_refl.
+
+    destruct (in_dec id_dec (getBlockLabel b0) rd).
+    Case "reachable".
+      remember
+        (pass.(iter_block)
+          (fdef_intro fh (bs1 ++ b0 :: bs2)) b0 ctx efs) as R.
+      destruct R as [[f' []] efs']; inv Hpass; eauto.
+        apply iter_block_unchanged in HeqR. destruct HeqR; subst.
+        iter_blocks_tac.
+    Case "unreachable". 
+      iter_blocks_tac.
+Qed.
+
+Lemma iter_blocks_sim_wfS': forall fh efs f0 efs0 main VarArgs flag bs
+  (Hpass:IterationPass.iter_blocks pass (fdef_intro fh bs) bs ctx 
+    rd efs = (f0, flag, efs0)) S1 S2
+  (Hrd: reachablity_analysis (fdef_intro fh bs) = Some rd)
+  (Heq1: S1 = [module_intro los nts (Ps1 ++  product_fdef f0 :: Ps2)])
+  (Heq2: S2 = [module_intro los nts (Ps1 ++ product_fdef (fdef_intro fh bs) :: Ps2)])
+  (HwfS : wf_system S2) (Hok: defined_program S2 main VarArgs), 
+  program_sim S1 S2 main VarArgs /\ wf_system S1 /\ defined_program S1 main VarArgs.
+Proof.
+  intros until bs.
+  rewrite_env (nil ++ bs).
+  intros. subst.
+  eapply iter_blocks_sim_wfS_aux'; eauto.
+Qed.
+
+Hypothesis iter_block_reachablity_successors: forall f b ctx f0
+  efs0 efs (Hpass : (f0, true, efs0) = pass.(iter_block) f b ctx efs),
+  reachablity_analysis f = reachablity_analysis f0 /\
+  successors f = successors f0.
+
+Lemma iter_wfS: forall f1 efs1 f2 efs2 main VarArgs
+  (Hpass: SafePrimIter.iterate _ (IterationPass.iter_step pass ctx rd) (f1, efs1) 
+    = (f2, efs2))
+  (Hrd: reachablity_analysis f1 = Some rd) S1 S2
+  (Heq1: S1 = [module_intro los nts (Ps1 ++ product_fdef f2 :: Ps2)])
+  (Heq2: S2 = [module_intro los nts (Ps1 ++ product_fdef f1 :: Ps2)])
+  (HwfS : wf_system S2) (Hok: defined_program S2 main VarArgs),
+  (program_sim S1 S2 main VarArgs /\ wf_system S1 /\
+    defined_program S1 main VarArgs) /\
+  reachablity_analysis f2 = reachablity_analysis f1 /\
+  successors f2 = successors f1.
+Proof.
+  intros. subst.
+  set (P:=fun (re:(fdef * pass.(effects))) =>
+          let '(f, _) := re in
+          (program_sim [module_intro los nts (Ps1 ++ product_fdef f :: Ps2)]
+            [module_intro los nts (Ps1 ++ product_fdef f1 :: Ps2)]
+            main VarArgs /\
+           wf_system
+            [module_intro los nts (Ps1 ++ product_fdef f :: Ps2)] /\
+           defined_program 
+            [module_intro los nts (Ps1 ++ product_fdef f :: Ps2)]
+            main VarArgs) /\
+         reachablity_analysis f = reachablity_analysis f1 /\
+         successors f = successors f1
+       ).
+  assert (P (f1, efs1)) as HPf1.
+    unfold P.
+    split; auto using program_sim_refl.
+  apply SafePrimIter.iterate_prop with (P:=P) in Hpass; auto.
+    unfold IterationPass.iter_step.
+    intros a HPa.
+    destruct a as [f efs].
+    unfold IterationPass.iter_fdef.
+    destruct f as [fh bs].
+    remember (IterationPass.iter_blocks pass (fdef_intro fh bs) bs 
+                ctx rd efs) as R.
+    destruct R as [[f0 flag0] efs0]; auto.
+    assert (P (f0, efs0)) as HPf0.
+      unfold P.
+      symmetry in HeqR.
+      destruct HPa as [[Hsima [HwfSa Hoka]] [Hreacha Hsucca]].
+      rewrite <- Hreacha in Hrd.
+      split.
+        apply program_sim_wfS_trans with (P2:=
+                [module_intro los nts
+                 (Ps1 ++ product_fdef (fdef_intro fh bs) :: Ps2)]); auto.
+        eapply iter_blocks_sim_wfS' in HeqR; eauto.
+
+        eapply iter_blocks_reachablity_successors in HeqR; eauto.
+        destruct HeqR. split; congruence.
+
+    destruct flag0; auto.
+Qed.
+
+End IterationPassSimWF.
+
+End IterationPassCorrect.
